Moved most of the stuff in concurrency/compiler/core_semantics.v into sepcomp/semantics.v, for compatibility with master branch.

concurrency/common/core_semantics.v
@@ -10,19 +10,7 @@ Require Import compcert.common.AST.
 Require Import compcert.common.Globalenvs.
 Require Import compcert.common.Smallstep.
 
-
-(** * Core Semantics *)
-
-Record CoreSemantics {C M : Type} : Type :=
-  { initial_core : nat -> M -> C -> M -> val -> list val -> Prop
-  ; at_external : C -> M -> option (external_function * list val)
-  ; after_external : option val -> C -> M -> option C
-  ; halted : C -> int -> Prop
-  ; corestep : C -> M -> C -> M -> Prop
-  ; corestep_not_halted:
-      forall m q m' q' i, corestep q m q' m' -> ~ halted q i
-  ; corestep_not_at_external:
-      forall m q m' q', corestep q m q' m' -> at_external q m = None }.
+Require Export VST.sepcomp.semantics.
 
 (* Extract a CoreSemantics from a part_semantics*)
 Inductive step2corestep (sem:part_semantics):(state sem) -> mem -> (state sem) -> mem -> Prop :=
@@ -31,7 +19,7 @@ Inductive step2corestep (sem:part_semantics):(state sem) -> mem -> (state sem) -
     Smallstep.at_external sem (set_mem s1 m1) = None ->
     step2corestep sem s1 m1 s2 (get_mem s2).
     
-Program Definition sem2coresem (sem:part_semantics) corestep_not_halted : CoreSemantics:=
+Program Definition sem2coresem (sem:part_semantics) corestep_not_halted : CoreSemantics _ _:=
   {|
     initial_core := fun _ m c m' f args => start_stack sem m c f args /\ get_mem c = m'
     ; at_external := fun s m => Smallstep.at_external sem (set_mem s m) 
@@ -43,44 +31,3 @@ Program Definition sem2coresem (sem:part_semantics) corestep_not_halted : CoreSe
 Next Obligation.
   inv H; auto.
 Qed.
-
-
-Arguments CoreSemantics : clear implicits.
-
-Inductive mem_step m m' : Prop :=
-    mem_step_storebytes: forall b ofs bytes,
-       Mem.storebytes m b ofs bytes = Some m' -> mem_step m m'
-  | mem_step_alloc: forall lo hi b',
-       Mem.alloc m lo hi = (m',b') -> mem_step m m'
-  | mem_step_freelist: forall l,
-       Mem.free_list m l = Some m' -> mem_step m m'
-  (*Some non-observable external calls are not a single alloc/free/store-step*)
-  | mem_step_trans: forall m'',
-       mem_step m m'' -> mem_step m'' m' -> mem_step m m'.
-
-Local Notation "a # b" := (PMap.get b a) (at level 1).
-Record perm_lesseq (m m': mem):= {
-  perm_le_Cur:
-    forall b ofs, Mem.perm_order'' ((Mem.mem_access m')#b ofs Cur) ((Mem.mem_access m)#b ofs Cur)
-; perm_le_Max:
-    forall b ofs, Mem.perm_order'' ((Mem.mem_access m')#b ofs Max) ((Mem.mem_access m)#b ofs Max)
-; perm_le_cont:
-    forall b ofs, Mem.perm m b ofs Cur Readable ->
-     ZMap.get ofs (Mem.mem_contents m') !! b= ZMap.get ofs (Mem.mem_contents m) !! b
-; perm_le_nb: Mem.nextblock m = Mem.nextblock m'
-}.
-
-
-(* Memory semantics are CoreSemantics that are specialized to CompCert memories
-   and evolve memory according to mem_step. Previous notion CoopCoreSem is deprecated,
-   but for now retained in file CoopCoreSem.v *)
-Record MemSem {C} :=
-  { csem :> @CoreSemantics C mem
-
-  ; corestep_mem : forall c m c' m' (CS: corestep csem c m c' m'), mem_step m m'
-  (*later, we'll want to add the following constraint
-  ; corestep_incr_perm: forall g c m c' m' (CS: corestep csem g c m c' m')  m1 (PLE: perm_lesseq m m1),
-         exists m1', corestep csem g c m1 c' m1' /\ perm_lesseq m' m1'*)
-  }.
-
-Arguments MemSem : clear implicits.
