sepcomp/step_lemmas.v
@@ -67,9 +67,10 @@ Section safety.
     inv H1; auto.
     erewrite corestep_not_at_external in H3; eauto; congruence.
     eapply safeN_halted; eauto.
-(*    erewrite corestep_not_halted in H2; eauto; congruence.
-  Qed.*)
-  Abort.
+    apply corestep_not_halted with (i0:=i) in H0. contradiction.
+    apply corestep_not_halted with (i0:=i) in H0. contradiction.
+  Unshelve. apply Integers.Int.zero.
+Qed.
 
   Lemma safe_corestep_backward:
     forall c m c' m' n z,
