veric/SeparationLogicSoundness.v
@@ -39,7 +39,7 @@ Axiom semax_prog_rule :
      Genv.init_mem prog = Some m ->
      { b : block & { q : corestate &
        (Genv.find_symbol (globalenv prog) (prog_main prog) = Some b) *
-       (forall jm, m_dry jm = m -> exists jm', core_semantics.initial_core (juicy_core_sem (cl_core_sem (globalenv prog))) h
+       (forall jm, m_dry jm = m -> exists jm', semantics.initial_core (juicy_core_sem (cl_core_sem (globalenv prog))) h
                     jm q jm' (Vptr b Ptrofs.zero) nil) *
        forall n, { jm |
        m_dry jm = m /\ level jm = n /\
@@ -57,7 +57,7 @@ Axiom semax_prog_rule' :
      Genv.init_mem prog = Some m ->
      { b : block & { q : corestate &
        (Genv.find_symbol (globalenv prog) (prog_main prog) = Some b) *
-       (forall jm, m_dry jm = m -> exists jm', core_semantics.initial_core (juicy_core_sem (cl_core_sem (globalenv prog))) h
+       (forall jm, m_dry jm = m -> exists jm', semantics.initial_core (juicy_core_sem (cl_core_sem (globalenv prog))) h
                     jm q jm' (Vptr b Ptrofs.zero) nil) *
        forall n z, { jm |
        m_dry jm = m /\ level jm = n /\
