veric/semax_lemmas.v
@@ -412,7 +412,7 @@ Proof.
   assert ((c',m') = (c'0,m'0)).
   { eapply juicy_core_sem_preserves_corestep_fun with (csem := cl_core_sem ge); eauto. }
   inv H0; auto.
-  setoid_rewrite (core_semantics.corestep_not_at_external (juicy_core_sem _)) in H2; eauto; congruence.
+  setoid_rewrite (semantics.corestep_not_at_external (juicy_core_sem _)) in H2; eauto; congruence.
   contradiction.
 Qed.
 
@@ -1496,7 +1496,7 @@ Focus 1.
   destruct l0; simpl in *.
   hnf in CS0.
   specialize (CS0 ora ve te m0 (S n)).
-  assert (core_semantics.corestep (juicy_core_sem (cl_core_sem ge)) (State ve te ctl1) m0 st' m'0).
+  assert (semantics.corestep (juicy_core_sem (cl_core_sem ge)) (State ve te ctl1) m0 st' m'0).
   split3; auto.
   pose proof (@jsafeN_step genv _ _ genv_symb_injective (cl_core_sem ge) OK_spec ge _ _ _ _ _ _ H5 H1).
   apply CS0 in H6; auto.
@@ -1514,7 +1514,7 @@ Focus 1.
   destruct l0; simpl in *.
   hnf in CS0.
   specialize (CS0 ora ve te m0 (S n)).
-  assert (core_semantics.corestep (juicy_core_sem (cl_core_sem ge)) (State ve te ctl1) m0 st' m'0).
+  assert (semantics.corestep (juicy_core_sem (cl_core_sem ge)) (State ve te ctl1) m0 st' m'0).
   split3; auto.
   pose proof (@jsafeN_step genv _ _ genv_symb_injective  (cl_core_sem ge) OK_spec ge _ _ _ _ _ _ H5 H1).
   apply CS0 in H6; auto.
